Examples/SQRL_Shorewall/Analyze_SQRL_Shorewall.thy
@@ -17,6 +17,8 @@ thm SQRL_fw_def
 
 thm SQRL_fw_FORWARD_default_policy_def
 
+value[code] "map (\<lambda>(c,rs). (c, map (quote_rewrite \<circ> common_primitive_rule_toString) rs)) SQRL_fw"
+
 lemma "Semantics_Goto.terminal_chain (the ((map_of_string SQRL_fw) ''smurflog''))" by eval
 lemma "Semantics_Goto.terminal_chain (the ((map_of_string SQRL_fw) ''logflags''))" by eval
 lemma "Semantics_Goto.terminal_chain (the ((map_of_string SQRL_fw) ''reject''))" by eval
